Tiny bit of progress on buftxn

src/program_proof/buftxn/idealized_buftxn_spec.v
@@ -2,10 +2,15 @@ From Perennial.algebra Require Import auth_map.
 From Perennial.algebra Require Import liftable.
 
 From Goose.github_com.mit_pdos.goose_nfsd Require Import buftxn.
-From Perennial.program_proof Require Import buf.buf_proof addr.addr_proof.
+From Perennial.program_proof Require Import buf.buf_proof addr.addr_proof txn.txn_proof.
+From Perennial.program_proof Require buftxn.buftxn_proof.
 From Perennial.program_proof Require Import proof_prelude.
 From Perennial.goose_lang.lib Require Import slice.typed_slice.
 From Perennial.goose_lang.ffi Require Import disk_prelude.
+
+(* mspec is a shorthand for referring to the old "map-based" spec, since we will
+want to use similar names in this spec *)
+Module mspec := buftxn.buftxn_proof.
 
 (* an object is the data for a sub-block object, a dynamic bundle of a kind and
 data of the appropriate size *)
@@ -23,17 +28,24 @@ Section goose_lang.
   Context `{!heapG Σ}.
   Context `{!buftxnG Σ}.
 
-  Implicit Types (l: loc) (γtxn γ: gname).
+  Implicit Types (l: loc) (γtxn: @txn_names Σ) (γ: gname).
   Implicit Types (obj: object).
 
   (* this is for the entire txn manager, and relates it to some ghost state *)
   Definition is_txn l γtxn : iProp Σ.
   Admitted.
 
-  (* TODO: this is complicated - it needs to assert ownership over a block in
-  the transaction system's abstract state (by instantiating the HOCAP P with
-  some auth state) but actually only assert ownership over a sub-block *)
-  Definition stable_maps_to γtxn (a: addr) obj: iProp Σ.
+  (* TODO: eventually need a proper name for this; I think of it as "the right
+  to use address [a] in a transaction", together with the fact that the current
+  disk value is obj *)
+  (* this is probably just [mspec.mapsto_txn] *)
+  Definition modify_token γtxn (a: addr) obj: iProp Σ.
+  Admitted.
+
+  (* TODO: I think this just connects to γUnified.(crash_states), which is the
+  name of an auth log_heap; when maintaining synchrony the ownership is really
+  simple since we only fully own the latest and forward value *)
+  Definition stable_maps_to γtxn (a:addr) obj: iProp Σ.
   Admitted.
 
   (* TODO: name this better *)
@@ -48,41 +60,43 @@ Section goose_lang.
 
   (* this is for a single buftxn (transaction) - not persistent, buftxn's are
   not shareable *)
-  Definition is_buftxn l (γtxn γ: gname) : iProp Σ :=
+  (* TODO: this is re-deriving mspec.is_buftxn; build directly on top, but
+  replace mT argument with a ghost name *)
+  Definition is_buftxn l γtxn γ : iProp Σ :=
     ∃ (txn_l: loc) (bufs_l: loc) (bufs: gmap addr buf),
       "txn" ∷ readonly (l ↦[BufTxn.S :: "txn"] #txn_l) ∗
       "bufs" ∷ readonly (l ↦[BufTxn.S :: "bufs"] #bufs_l) ∗
       "Htxn" ∷ is_txn txn_l γtxn ∗
       "Hbufs" ∷ is_bufmap bufs_l bufs ∗
       "Hctx" ∷ buftxn_ctx γ bufs ∗
-      "Hold_stable" ∷ ([∗ map] a↦_ ∈ bufs, ∃ obj0, stable_maps_to γtxn a obj0).
+      "Hold_stable" ∷ ([∗ map] a↦_ ∈ bufs, ∃ obj0, modify_token γtxn a obj0).
 
   Definition buftxn_maps_to γ (a: addr) obj : iProp Σ :=
     ∃ q, ptsto γ a q obj.
 
   Theorem lift_into_txn γtxn γ bufs a obj :
     buftxn_ctx γ bufs -∗
-    stable_maps_to γtxn a obj ==∗
+    modify_token γtxn a obj ==∗
     buftxn_maps_to γ a obj ∗ buftxn_ctx γ bufs.
   Proof.
-    (* TODO: allocate into buftxn_ctx, consume stable_maps_to into
+    (* TODO: allocate into buftxn_ctx, consume modify_token into
     buftxn_ctx *)
   Admitted.
 
-  Lemma stable_maps_to_conflicting γtxn :
-    Conflicting (stable_maps_to γtxn) (stable_maps_to γtxn).
+  Lemma modify_token_conflicting γtxn :
+    Conflicting (modify_token γtxn) (modify_token γtxn).
   Proof.
   Admitted.
 
   Theorem lift_liftable_into_txn `{!Liftable P}
           γtxn γ bufs :
     buftxn_ctx γ bufs -∗
-    P (stable_maps_to γtxn) ==∗
+    P (modify_token γtxn) ==∗
     P (buftxn_maps_to γ) ∗ buftxn_ctx γ bufs.
   Proof.
     iIntros "Hctx HP".
     iDestruct (liftable (P:=P) with "HP") as (m) "[Hm HP]".
-    { apply stable_maps_to_conflicting. }
+    { apply modify_token_conflicting. }
     iSpecialize ("HP" $! (buftxn_maps_to γ)).
     iInduction m as [|i x m] "IH" using map_ind.
     - iModIntro.
@@ -129,6 +143,22 @@ Section goose_lang.
     {{{ is_buftxn l γtxn γ ∗ buftxn_maps_to γ a obj0 ∗ is_slice data_s byteT q data }}}
       BufTxn__OverWrite #l (addr2val a) (slice_val data_s)
     {{{ RET #(); buftxn_maps_to γ a obj }}}.
+  Proof.
+  Admitted.
+
+  (* TODO: almost certainly wrong in some fundamental way *)
+  (* the idea is that the caller gets to open an invariant and extract an old
+  version of whatever they've modified, then substitute it for a newly-prepared
+  transaction *)
+  (* eventually we need to correlate the footprints of these lifted
+  predicates; TODO: won't it be difficult to establish that the footprint of P
+  hasn't changed in the invariant? it hasn't because we've had it locked, but we
+  don't have ownership over it... *)
+  Theorem wp_BufTxn__CommitWait l γtxn γ E `{!Liftable P0, !Liftable P} Q :
+    {{{ is_buftxn l γtxn γ ∗ P (buftxn_maps_to γ) ∗
+        |={⊤,E}=> (P0 (stable_maps_to γtxn) ∗ (P (stable_maps_to γtxn) ={E,⊤}=∗ Q))  }}}
+      BufTxn__CommitWait #l #true
+    {{{ (n:u64), RET #n; Q }}}.
   Proof.
   Admitted.
 
